Do not use keys to represent principals.
Up till now, resources such as keys and nonces had to carry which encryption
keys could be used to declassify them to public.  This required a complicated
invariant for resources to be well-formed: a principal, represented as a key,
had to ensure that all of this keys readers were not public.

I decided to replace this by a simpler public/secret distinction.  The hope is
that this will make it easier to verify protocols without forcing all
participants to be honest.

crypto1.v
@@ -105,33 +105,83 @@ Instance readers_unit : Unit readers := RPriv ∅.
 Lemma readers_ucmra_mixin : UcmraMixin readersR.
 Proof. split=> //; case=> // rs; congr RPriv; set_solver+. Qed.
 
+Section Levels.
+
+Inductive level := Pub | Sec.
+
+Canonical levelO := leibnizO level.
+
+Implicit Types lvl : level.
+
+Global Instance level_sqsubseteq : SqSubsetEq level := λ lvl1 lvl2,
+  match lvl1, lvl2 with
+  | Sec, Pub => False
+  | _, _ => True
+  end.
+
+Global Instance level_sqsubseteq_refl : Reflexive level_sqsubseteq.
+Proof. by case. Qed.
+
+Global Instance level_sqsubseteq_tran : Transitive level_sqsubseteq.
+Proof. by case=> [] [] []. Qed.
+
+Global Instance level_join : Join level := λ lvl1 lvl2,
+  match lvl1, lvl2 with
+  | Pub, Pub => Pub
+  | _, _ => Sec
+  end.
+
+Lemma level_joinP lvl1 lvl2 lvl3 :
+  lvl1 ⊔ lvl2 ⊑ lvl3 ↔ (lvl1 ⊑ lvl3 ∧ lvl2 ⊑ lvl3).
+Proof.
+by case: lvl1 lvl2 lvl3=> [] [] []; intuition eauto.
+Qed.
+
+Global Instance level_meet : Meet level := λ lvl1 lvl2,
+  match lvl1, lvl2 with
+  | Sec, Sec => Sec
+  | _, _ => Pub
+  end.
+
+Lemma level_meetP lvl1 lvl2 lvl3 :
+  lvl3 ⊑ lvl1 ⊓ lvl2 ↔ (lvl3 ⊑ lvl1 ∧ lvl3 ⊑ lvl2).
+Proof.
+by case: lvl1 lvl2 lvl3=> [] [] []; intuition eauto.
+Qed.
+
+Global Instance level_inhabited : Inhabited level :=
+  populate Pub.
+
+End Levels.
+
 Section Resources.
 
 Context (Σ : gFunctors).
 Implicit Types Φ : termO -n> iPropO Σ.
 Implicit Types l : loc.
+Implicit Types lvl : level.
 Implicit Types γ : gname.
 
 Inductive res :=
-| RNonce of readers
-| RAKey of readers & readers & termO -n> iPropO Σ
-| RSKey of readers & termO -n> iPropO Σ.
+| RNonce of level
+| RAKey of level & level & termO -n> iPropO Σ
+| RSKey of level & termO -n> iPropO Σ.
 
 Global Instance res_equiv : Equiv res := λ r1 r2,
   match r1, r2 with
-  | RNonce rs1, RNonce rs2 => rs1 = rs2
-  | RAKey rs11 rs12 P1, RAKey rs21 rs22 P2 =>
-    rs11 = rs21 ∧ rs12 = rs22 ∧ P1 ≡ P2
-  | RSKey rs1 P1, RSKey rs2 P2 => rs1 = rs2 ∧ P1 ≡ P2
+  | RNonce lvl1, RNonce lvl2 => lvl1 = lvl2
+  | RAKey lvl11 lvl12 P1, RAKey lvl21 lvl22 P2 =>
+    lvl11 = lvl21 ∧ lvl12 = lvl22 ∧ P1 ≡ P2
+  | RSKey lvl1 P1, RSKey lvl2 P2 => lvl1 = lvl2 ∧ P1 ≡ P2
   | _, _ => False
   end.
 
 Global Instance res_dist : Dist res := λ n r1 r2,
   match r1, r2 with
-  | RNonce rs1, RNonce rs2 => rs1 = rs2
-  | RAKey rs11 rs12 P1, RAKey rs21 rs22 P2 =>
-    rs11 = rs21 ∧ rs12 = rs22 ∧ P1 ≡{n}≡ P2
-  | RSKey rs1 P1, RSKey rs2 P2 => rs1 = rs2 ∧ P1 ≡{n}≡ P2
+  | RNonce lvl1, RNonce lvl2 => lvl1 = lvl2
+  | RAKey lvl11 lvl12 P1, RAKey lvl21 lvl22 P2 =>
+    lvl11 = lvl21 ∧ lvl12 = lvl22 ∧ P1 ≡{n}≡ P2
+  | RSKey lvl1 P1, RSKey lvl2 P2 => lvl1 = lvl2 ∧ P1 ≡{n}≡ P2
   | _, _ => False
   end.
 
@@ -143,7 +193,7 @@ split.
   intuition eauto using 0.
 - rewrite /dist; move=> n; split.
   + case=> * //=; by apply equiv_dist.
-  + case=> [rs1|rs11 rs12 P1|rs1 P1] [rs2|rs21 rs22 P2|rs2 P2] //=;
+  + case=> [lvl1|lvl11 lvl12 P1|lvl1 P1] [lvl2|lvl21 lvl22 P2|lvl2 P2] //=;
     intuition eauto.
   + case=> [?|???|??] [?|???|??] //= [?|???|??] //=;
     intuition (try congruence); etransitivity; eauto.
@@ -155,35 +205,17 @@ Canonical resO := OfeT res res_ofe_mixin.
 Lemma res_equivI (r1 r2 : res) :
   r1 ≡ r2 ⊣⊢@{iPropI Σ}
   match r1, r2 with
-  | RNonce rs1, RNonce rs2 => ⌜rs1 = rs2⌝
-  | RAKey rs_enc1 rs_dec1 Φ1, RAKey rs_enc2 rs_dec2 Φ2 =>
-    ⌜rs_enc1 = rs_enc2⌝ ∧ ⌜rs_dec1 = rs_dec2⌝ ∧ Φ1 ≡ Φ2
-  | RSKey rs1 Φ1, RSKey rs2 Φ2 =>
-    ⌜rs1 = rs2⌝ ∧ Φ1 ≡ Φ2
+  | RNonce lvl1, RNonce lvl2 => ⌜lvl1 = lvl2⌝
+  | RAKey lvl_enc1 lvl_dec1 Φ1, RAKey lvl_enc2 lvl_dec2 Φ2 =>
+    ⌜lvl_enc1 = lvl_enc2⌝ ∧ ⌜lvl_dec1 = lvl_dec2⌝ ∧ Φ1 ≡ Φ2
+  | RSKey lvl1 Φ1, RSKey lvl2 Φ2 =>
+    ⌜lvl1 = lvl2⌝ ∧ Φ1 ≡ Φ2
   | _, _ => False
   end.
 Proof. case: r1=> *; case: r2=> * /=; by uPred.unseal. Qed.
 
-Global Instance discrete_RNonce rs : Discrete (RNonce rs).
+Global Instance discrete_RNonce lvl : Discrete (RNonce lvl).
 Proof. by case. Qed.
-
-Definition priv_dec_key (rs : gset loc) r : Prop :=
-  match r with
-  | RAKey _ (RPriv rs') _ | RSKey (RPriv rs') _ => rs' ⊆ rs
-  | _ => False
-  end.
-
-Lemma priv_dec_key_sub rs rs' r :
-  rs ⊆ rs' → priv_dec_key rs r → priv_dec_key rs' r.
-Proof.
-case: r=> [?|?[|?]?|[|?]?] //=; set_solver.
-Qed.
-
-Definition pub_dec_key r : Prop :=
-  match r with
-  | RAKey _ RPub _ | RSKey RPub _ => True
-  | _ => False
-  end.
 
 Class resG := {
   res_inG :> inG Σ (agreeR resO);
@@ -191,13 +223,13 @@ Class resG := {
 
 Context `{!resG, !heapG Σ}.
 
-Definition pre_resT r l : iProp Σ :=
+Definition resT r l : iProp Σ :=
   ∃ γ, meta l (cryptoN.@"res") γ ∗ own γ (to_agree r).
 
-Lemma pre_resT_persistent r l : Persistent (pre_resT r l).
+Lemma resT_persistent r l : Persistent (resT r l).
 Proof. apply _. Qed.
 
-Lemma pre_resT_agree r1 r2 l : pre_resT r1 l -∗ pre_resT r2 l -∗ r1 ≡ r2.
+Lemma resT_agree r1 r2 l : resT r1 l -∗ resT r2 l -∗ r1 ≡ r2.
 Proof.
 iDestruct 1 as (γ) "[#Hl #Hγ]".
 iDestruct 1 as (γ') "[#Hl' #Hγ']".
@@ -206,8 +238,8 @@ iPoseProof (own_valid_2 with "Hγ Hγ'") as "Hvalid".
 by rewrite agree_validI agree_equivI.
 Qed.
 
-Lemma later_pre_resT r l :
-  ▷ pre_resT r l -∗ ◇ ∃ r', pre_resT r' l ∗ ▷ (r ≡ r').
+Lemma later_resT r l :
+  ▷ resT r l -∗ ◇ ∃ r', resT r' l ∗ ▷ (r ≡ r').
 Proof.
 iDestruct 1 as (γ) "[> #Hmeta Hown]".
 iMod (later_own with "Hown") as (ag) "[#Hown #Hr]".
@@ -218,212 +250,32 @@ iModIntro; iExists r'; iSplit=> //.
 by iExists γ; iSplit.
 Qed.
 
-Definition pre_wf_readers rs_priv rs :=
-  match rs with
-  | RPub     => True
-  | RPriv rs => rs ⊆ rs_priv
-  end.
+Definition nonceT lvl l : iProp Σ := resT (RNonce lvl) l.
 
-Lemma pre_wf_readers_sub rs_priv rs_priv' rs :
-  rs_priv ⊆ rs_priv' → pre_wf_readers rs_priv rs → pre_wf_readers rs_priv' rs.
-Proof. case: rs=> //= rs *; set_solver. Qed.
-
-Definition pre_wf_res rs_priv r :=
-  match r with
-  | RNonce rs => pre_wf_readers rs_priv rs
-  | RAKey rs1 rs2 _ => pre_wf_readers rs_priv rs1 ∧ pre_wf_readers rs_priv rs2
-  | RSKey rs _ => pre_wf_readers rs_priv rs
-  end.
-
-Definition priv_keyT rs_priv l : iProp Σ :=
-  ∃ r, pre_resT r l ∗ ⌜priv_dec_key rs_priv r⌝.
-
-Global Instance priv_keyT_proper :
-  Proper (equiv ==> equiv ==> equiv) priv_keyT.
-Proof.
-by move=> rs1 rs2 /(leibniz_equiv rs1 rs2) -> l1 l2 /(leibniz_equiv l1 l2) ->.
-Qed.
-
-Global Instance priv_keyT_ne : NonExpansive2 priv_keyT.
-Proof.
-move=> n.
-by move=> rs1 rs2 /(leibniz_equiv rs1 rs2) -> l1 l2 /(leibniz_equiv l1 l2) ->.
-Qed.
-
-Global Instance priv_keyT_persistent rs_priv l :
-  Persistent (priv_keyT rs_priv l).
-Proof. apply _. Qed.
-
-Global Instance priv_keyT_timeless rs_priv l :
-  Timeless (priv_keyT rs_priv l).
-Proof.
-rewrite /Timeless /priv_keyT bi.later_exist_except_0.
-iMod 1 as (r) "[#Hown >%Hpriv]".
-iMod (later_pre_resT with "Hown") as (r') "[Hown' He]".
-iExists r'; iSplit; eauto; rewrite res_equivI.
-case: r Hpriv => [rs|rs_enc [|rs_dec] Φ|[|rs_dec] Φ] //= Hpriv;
-case: r'=> [?|???|??]; try by iDestruct "He" as "> []".
-- by iDestruct "He" as "(><-&><-&?)".
-- by iDestruct "He" as "(><-&?)".
-Qed.
-
-Lemma priv_keyT_sub rs_priv rs_priv' l :
-  rs_priv ⊆ rs_priv' → priv_keyT rs_priv l -∗ priv_keyT rs_priv' l.
-Proof.
-move=> sub; iDestruct 1 as (r) "[Hr %Hpriv]".
-iExists r; iFrame; iPureIntro.
-by eapply priv_dec_key_sub.
-Qed.
-
-Definition priv_keysT rs_priv : iProp Σ :=
-  ∀ l, ⌜l ∈ rs_priv⌝ -∗ priv_keyT rs_priv l.
-
-Definition pub_keyT l : iProp Σ :=
-  ∃ r, pre_resT r l ∗ ⌜pub_dec_key r⌝.
-
-Global Instance pub_keyT_persistent l : Persistent (pub_keyT l).
-Proof. apply _. Qed.
-
-Global Instance pub_keyT_timeless l : Timeless (pub_keyT l).
-Proof.
-rewrite /Timeless /pub_keyT bi.later_exist_except_0.
-iMod 1 as (r) "[#Hown >%Hpriv]".
-iMod (later_pre_resT with "Hown") as (r') "[Hown' He]".
-iExists r'; iSplit; eauto; rewrite res_equivI.
-case: r Hpriv => [rs|rs_enc [|rs_dec] Φ|[|rs_dec] Φ] //= Hpriv;
-case: r'=> [?|???|??]; try by iDestruct "He" as "> []".
-- by iDestruct "He" as "(><-&><-&?)".
-- by iDestruct "He" as "(><-&?)".
-Qed.
-
-Definition pub_keysT (rs_pub : gset loc) : iProp Σ :=
-  ∀ l, ⌜l ∈ rs_pub⌝ -∗ pub_keyT l.
-
-Global Instance pub_keysT_persistent rs_pub : Persistent (pub_keysT rs_pub).
-Proof. apply _. Qed.
-
-Global Instance pub_keysT_timeless rs_pub : Timeless (pub_keysT rs_pub).
-Proof. apply _. Qed.
-
-Definition wf_readers_priv rs : iProp Σ :=
-  ∃ rs_priv, priv_keysT rs_priv ∗ ⌜pre_wf_readers rs_priv rs⌝.
-
-Global Instance wf_readers_priv_persistent rs : Persistent (wf_readers_priv rs).
-Proof. apply _. Qed.
-
-Global Instance wf_readers_priv_timeless rs : Timeless (wf_readers_priv rs).
-Proof. apply _. Qed.
-
-Definition wf_readers rs : iProp Σ :=
-  match rs with
-  | RPub => True
-  | RPriv rs =>
-    ∃ rs1 rs2, ⌜rs = rs1 ∪ rs2⌝ ∗ wf_readers_priv (RPriv rs1) ∗ pub_keysT rs2
-  end.
-
-Global Instance wf_readers_persistent rs : Persistent (wf_readers rs).
-Proof. case: rs=> *; apply _. Qed.
-
-Global Instance wf_readers_timeless rs : Timeless (wf_readers rs).
-Proof. case: rs=> *; apply _. Qed.
-
-Definition wf_res_priv r : iProp Σ :=
-  ∃ rs_priv, priv_keysT rs_priv ∗ ⌜pre_wf_res rs_priv r⌝.
-
-Global Instance wf_res_priv_persistent r : Persistent (wf_res_priv r).
-Proof. apply _. Qed.
-
-Global Instance wf_res_priv_timeless r : Timeless (wf_res_priv r).
-Proof. apply _. Qed.
-
-Lemma wf_res_privE r :
-  wf_res_priv r ⊣⊢@{iPropI Σ}
-  match r with
-  | RNonce rs => wf_readers_priv rs
-  | RAKey rs_enc rs_dec _ => wf_readers_priv rs_enc ∧ wf_readers_priv rs_dec
-  | RSKey rs _ => wf_readers_priv rs
-  end.
-Proof.
-case: r; try by move=> *; iSplit; eauto.
-move=> rs_enc rs_dec Φ /=; iSplit.
-- iDestruct 1 as (rs_priv) "(wf_rs_priv & %wf_rs_enc & %wf_rs_dec)".
-  by iSplit; iExists rs_priv; iSplit.
-- iIntros "[Henc Hdec]".
-  iDestruct "Henc" as (rs_priv_enc) "[Hpriv_enc %Hwf_enc]".
-  iDestruct "Hdec" as (rs_priv_dec) "[Hpriv_dec %Hwf_dec]".
-  iExists (rs_priv_enc ∪ rs_priv_dec); iSplit; last first.
-    iPureIntro; split; eapply pre_wf_readers_sub; try eassumption;
-    set_solver.
-  iIntros (l) "%Hl"; case/elem_of_union: Hl=> Hl.
-  + iSpecialize ("Hpriv_enc" $! _ Hl).
-    iApply (priv_keyT_sub with "Hpriv_enc"); set_solver.
-  + iSpecialize ("Hpriv_dec" $! _ Hl).
-    iApply (priv_keyT_sub with "Hpriv_dec"); set_solver.
-Qed.
-
-Definition res_privT r l : iProp Σ :=
-  pre_resT r l ∗ wf_res_priv r.
-
-Lemma res_privT_agree r1 r2 l : res_privT r1 l -∗ res_privT r2 l -∗ r1 ≡ r2.
-Proof.
-iIntros "[Hr1 _] [Hr2 _]". iApply (pre_resT_agree with "Hr1 Hr2").
-Qed.
-
-Global Instance res_privT_persistent r l : Persistent (res_privT r l).
-Proof. apply _. Qed.
-
-Definition wf_res r : iProp Σ :=
-  match r with
-  | RNonce rs => wf_readers rs
-  | RAKey rs_enc rs_dec _ => wf_readers rs_enc ∧ wf_readers rs_dec
-  | RSKey rs _ => wf_readers rs
-  end.
-
-Global Instance wf_resT_persistent r : Persistent (wf_res r).
-Proof. case: r=> *; apply _. Qed.
-
-Global Instance wf_resT_timeless r : Timeless (wf_res r).
-Proof. case: r=> *; apply _. Qed.
-
-Definition resT r l : iProp Σ :=
-  pre_resT r l ∗ wf_res r.
-
-Lemma resT_agree r1 r2 l : resT r1 l -∗ resT r2 l -∗ r1 ≡ r2.
-Proof.
-iIntros "[Hr1 _] [Hr2 _]". iApply (pre_resT_agree with "Hr1 Hr2").
-Qed.
-
-Global Instance resT_persistent r l : Persistent (resT r l).
-Proof. case: r=> *; apply _. Qed.
-
-Definition nonceT rs l : iProp Σ := resT (RNonce rs) l.
-
-Lemma nonceT_agree rs1 rs2 l : nonceT rs1 l -∗ nonceT rs2 l -∗ ⌜rs1 = rs2⌝.
+Lemma nonceT_agree lvl1 lvl2 l : nonceT lvl1 l -∗ nonceT lvl2 l -∗ ⌜lvl1 = lvl2⌝.
 Proof.
 iIntros "Hown1 Hown2".
 iPoseProof (resT_agree with "Hown1 Hown2") as "#Hvalid".
 by rewrite res_equivI.
 Qed.
 
-Global Instance persistent_nonceT rs l :
-  Persistent (nonceT rs l).
+Global Instance persistent_nonceT lvl l : Persistent (nonceT lvl l).
 Proof. apply _. Qed.
 
-Global Instance timeless_nonceT rs l :
-  Timeless (nonceT rs l).
+Global Instance timeless_nonceT lvl l : Timeless (nonceT lvl l).
 Proof. apply _. Qed.
 
-Definition akeyT rs_enc rs_dec Φ l : iProp Σ :=
-  resT (RAKey rs_enc rs_dec Φ) l.
+Definition akeyT lvl_enc lvl_dec Φ l : iProp Σ :=
+  resT (RAKey lvl_enc lvl_dec Φ) l.
 
-Global Instance persistent_akeyT rs_enc rs_dec Φ l :
-  Persistent (akeyT rs_enc rs_dec Φ l).
+Global Instance persistent_akeyT lvl_enc lvl_dec Φ l :
+  Persistent (akeyT lvl_enc lvl_dec Φ l).
 Proof. apply _. Qed.
 
-Definition skeyT rs Φ l : iProp Σ := resT (RSKey rs Φ) l.
+Definition skeyT lvl Φ l : iProp Σ := resT (RSKey lvl Φ) l.
 
-Global Instance persistent_skeyT rs Φ l :
-  Persistent (skeyT rs Φ l).
+Global Instance persistent_skeyT lvl Φ l :
+  Persistent (skeyT lvl Φ l).
 Proof. apply _. Qed.
 
 Definition keyT kt rs Φ l : iProp Σ :=
@@ -455,30 +307,59 @@ Qed.
 Global Instance persistent_keyT kt rs Φ l : Persistent (keyT kt rs Φ l).
 Proof. by case: kt; apply _. Qed.
 
-(** [termT rs t] holds when the term [t] can be declared public after encrypting
-it with any of the readers rs.  If [rs = RPub], [t] is considered public and
-does not have to be encrypted. *)
+Definition key_info (asym : bool) lvl_enc lvl_dec Φ l : iProp Σ :=
+  if asym then akeyT lvl_enc lvl_dec Φ l
+  else (⌜lvl_enc = lvl_dec⌝ ∗ skeyT lvl_enc Φ l)%I.
 
-Fixpoint termT rs t : iProp Σ :=
+Lemma key_info_agree asym1 asym2 lvl_enc1 lvl_dec1 lvl_enc2 lvl_dec2  Φ1 Φ2 l :
+  key_info asym1 lvl_enc1 lvl_dec1 Φ1 l -∗
+  key_info asym2 lvl_enc2 lvl_dec2 Φ2 l -∗
+  ⌜asym1 = asym2⌝ ∗ ⌜lvl_enc1 = lvl_enc2⌝ ∗ ⌜lvl_dec1 = lvl_dec2⌝ ∗ Φ1 ≡ Φ2.
+Proof.
+case: asym1 asym2=> [] [] /=.
+- iIntros "Hown1 Hown2".
+  iPoseProof (resT_agree with "Hown1 Hown2") as "#Hvalid".
+  by rewrite res_equivI /=; iDestruct "Hvalid" as "(?&?&?)"; repeat iSplit.
+- iIntros "Hown1 [_ Hown2]".
+  iPoseProof (resT_agree with "Hown1 Hown2") as "#Hvalid".
+  by rewrite res_equivI.
+- iIntros "[_ Hown1] Hown2".
+  iPoseProof (resT_agree with "Hown1 Hown2") as "#Hvalid".
+  by rewrite res_equivI.
+- iIntros "[<- Hown1] [<- Hown2]".
+  iPoseProof (resT_agree with "Hown1 Hown2") as "#Hvalid".
+  by rewrite res_equivI /=; iDestruct "Hvalid" as "(?&?)"; repeat iSplit.
+Qed.
+
+Global Instance persistent_key_info asym lvl_enc lvl_dec Φ l :
+  Persistent (key_info asym lvl_enc lvl_dec Φ l).
+Proof. by case: asym; apply _. Qed.
+
+(** [termT lvl t] holds when the term [t] can be declared public after
+encrypting it with any of the readers lvl.  If [lvl = Pub], [t] is considered
+public and does not have to be encrypted. *)
+
+Fixpoint termT lvl t : iProp Σ :=
   match t with
   | TInt _ => True
-  | TPair t1 t2 => termT rs t1 ∗ termT rs t2
-  | TNonce l  => ∃ rs', nonceT rs' l ∗ ⌜rs ⊆ rs'⌝
-  | TKey kt l => ∃ rs' Φ, keyT kt rs' Φ l ∗ ⌜rs ⊆ rs'⌝
+  | TPair t1 t2 => termT lvl t1 ∗ termT lvl t2
+  | TNonce l  => ∃ lvl', nonceT lvl' l ∗ ⌜lvl' ⊑ lvl⌝
+  | TKey kt l => ∃ lvl' Φ, keyT kt lvl' Φ l ∗ ⌜lvl' ⊑ lvl⌝
   | TEnc asym l t =>
-    let kt := if asym then KAEnc else KSym in
-    ∃ rs' Φ, keyT kt rs' Φ l
-             ∗ (□ Φ t ∗ termT {[l]} t ∨ ⌜rs' = RPub⌝ ∗ termT RPub t)
+    ∃ lvl_enc lvl_dec Φ,
+      key_info asym lvl_enc lvl_dec Φ l
+      ∗ (□ Φ t ∗ termT (lvl ⊔ lvl_dec) t ∨
+         ⌜lvl_enc = Pub⌝ ∗ termT Pub t)
   end.
 
-Global Instance persistent_termT rs t :
-  Persistent (termT rs t).
-Proof. elim: t rs=> *; apply _. Qed.
+Global Instance persistent_termT lvl t :
+  Persistent (termT lvl t).
+Proof. elim: t lvl=> *; apply _. Qed.
 
-Lemma term_proj_termT t n rs t' :
-  term_proj t n = Some t' →
-  termT rs t -∗
-  termT rs t'.
+Lemma proj_termT t n lvl t' :
+  Spec.proj t n = Some t' →
+  termT lvl t -∗
+  termT lvl t'.
 Proof.
 elim: t n=> // t1 IH1 t2 IH2 [|n] /=.
   by move=> [<-]; iIntros "[??]".
@@ -486,67 +367,40 @@ move=> {}/IH2 IH2; iIntros "[??]".
 by iApply IH2.
 Qed.
 
-Lemma sub_termT rs rs' t :
-  rs' ⊆ rs →
-  termT rs t -∗
-  termT rs' t.
+Lemma sub_termT lvl lvl' t :
+  lvl ⊑ lvl' →
+  termT lvl t -∗
+  termT lvl' t.
 Proof.
-elim: t rs=> [n|t1 IH1 t2 IH2|l|kt l|b l t IH] rs sub //=.
+elim: t lvl lvl'=> [n|t1 IH1 t2 IH2|l|kt l|b l t IH] lvl lvl' sub //=.
 - by iIntros "[#Ht1 #Ht2]"; rewrite IH1 // IH2 //; iSplit.
-- iDestruct 1 as (rs0) "[#Hnonce %sub0]".
-  iExists rs0; iSplit=> //; iPureIntro; by etransitivity.
-- iDestruct 1 as (rs0 Φ) "[#Hkey %sub0]".
-  iExists rs0, Φ; iSplit=> //; iPureIntro; by etransitivity.
+- iDestruct 1 as (lvl0) "[#Hnonce %sub0]".
+  iExists lvl0; iSplit=> //; iPureIntro; by etransitivity.
+- iDestruct 1 as (lvl0 Φ) "[#Hkey %sub0]".
+  iExists lvl0, Φ; iSplit=> //; iPureIntro; by etransitivity.
+- iDestruct 1 as (lvl_enc lvl_dec Φ) "[#Hkey #Ht]".
+  iExists lvl_enc, lvl_dec, Φ; iSplit=> //.
+  iDestruct "Ht" as "[[? Ht]|Ht]"; last by iRight.
+  iLeft; iSplit=> //; iApply (IH with "Ht").
+  by case: lvl lvl' lvl_dec sub=> [] [] [].
 Qed.
 
 (** A stricter version of [termT] that does not allow subtyping *)
-Definition stermT rs t : iProp Σ :=
-  termT rs t ∗ □ (∀ rs', termT rs' t -∗ ⌜rs' ⊆ rs⌝).
+Definition stermT lvl t : iProp Σ :=
+  termT lvl t ∗ □ (∀ lvl', termT lvl' t -∗ ⌜lvl ⊑ lvl'⌝).
 
-Global Instance stermT_persistent rs t : Persistent (stermT rs t).
+Global Instance stermT_persistent lvl t : Persistent (stermT lvl t).
 Proof. apply _. Qed.
-
-Definition termT' rs t : iProp Σ :=
-  termT rs t ∨ ∃ l, ⌜l ∈ rs⌝ ∗ pub_keyT l ∗ termT RPub t.
-
-Definition stermT' rs t : iProp Σ :=
-  stermT rs t ∨ ∃ l, ⌜l ∈ rs⌝ ∗ pub_keyT l ∗ termT RPub t.
-
-(** Because of [sub_termT], the definition of [termT] does not allow us to track
-the owners of a term exactly.  To remedy that, we introduce the [secretT rs t]
-predicate below, which says that [t] is private exactly to the readers in
-[rs].  *)
-
-Fixpoint secretT_def (rs : gset loc) t : iProp Σ :=
-  match t with
-  | TInt _ => False
-  | TPair t1 t2 => secretT_def rs t1 ∨ secretT_def rs t2
-  | TNonce l => nonceT (RPriv rs) l
-  | TKey kt l => ∃ Φ, keyT kt (RPriv rs) Φ l
-  | TEnc _ _ _ => False
-  end.
-
-Global Instance secretT_def_persistent (rs : gset loc) t :
-  Persistent (secretT_def rs t).
-Proof. by elim: t=> *; apply _. Qed.
-
-Definition secretT (rs : gset loc) t : iProp Σ :=
-  termT (RPriv rs) t ∗ secretT_def rs t.
-
-Global Instance secretT_persistent (rs : gset loc) t :
-  Persistent (secretT rs t).
-Proof. by apply _. Qed.
 
 Lemma res_alloc E r l :
   ↑cryptoN.@"res" ⊆ E →
-  meta_token l E -∗
-  wf_res r ==∗
+  meta_token l E ==∗
   resT r l.
 Proof.
-iIntros (Hsub) "Hmeta #Hr".
+iIntros (Hsub) "Hmeta".
 iMod (own_alloc (to_agree r)) as (γ) "#Hown" => //.
 iMod (meta_set E l γ with "Hmeta") as "Hmeta"=> //.
-by iModIntro; iSplit=> //; iExists γ; iSplit.
+by iModIntro; iExists γ; iSplit.
 Qed.
 
 End Resources.
@@ -555,7 +409,3 @@ Arguments RNonce {_} _.
 Arguments nonceT {_ _ _} _ _.
 Arguments skeyT {_ _ _} _ _ _.
 Arguments akeyT {_ _ _} _ _ _ _.
-Arguments wf_readers_priv {_ _ _} _.
-Arguments wf_readers {_ _ _} _.
-Arguments wf_res_priv {_ _ _} _.
-Arguments wf_res {_ _ _} _.
