term.v
@@ -43,6 +43,8 @@ Proof. by apply (@cancel_inj _ _ _ key_type_of_int); apply _. Qed.
 Instance int_of_key_type_countable : Countable key_type.
 Proof. apply (inj_countable' _ _ int_of_key_typeK). Qed.
 
+Instance repr_key_type : Repr key_type := λ kt, #(int_of_key_type kt).
+
 Inductive term  :=
 | TInt of Z
 | TPair of term & term
@@ -57,13 +59,6 @@ Notation TPair_tag := 1%Z.
 Notation TNonce_tag := 2%Z.
 Notation TKey_tag := 3%Z.
 Notation TEnc_tag := 4%Z.
-
-Fixpoint term_proj t n {struct t} :=
-  match t, n with
-  | TPair t _, 0 => Some t
-  | TPair _ t, S n => term_proj t n
-  | _, _ => None
-  end.
 
 Global Instance term_eq_dec : EqDecision term.
 Proof.
@@ -97,7 +92,7 @@ Definition val_of_term := locked val_of_term_rec.
 Lemma val_of_termE : val_of_term = val_of_term_rec.
 Proof. by rewrite /val_of_term -lock. Qed.
 Coercion val_of_term : term >-> val.
-Instance repr_term : Repr term := val_of_term.
+Global Instance repr_term : Repr term := val_of_term.
 
 Fixpoint term_of_val v : term :=
   match v with
@@ -136,3 +131,35 @@ Fixpoint symbols_of_term t : gset loc :=
   | TKey _ l => {[l]}
   | TEnc _ l t => {[l]} ∪ symbols_of_term t
   end.
+
+Module Spec.
+
+Fixpoint proj t n {struct t} :=
+  match t, n with
+  | TPair t _, 0 => Some t
+  | TPair _ t, S n => proj t n
+  | _, _ => None
+  end.
+
+Definition enc k t : option term :=
+  match k with
+  | TKey KSym l => Some (TEnc false l t)
+  | TKey KAEnc l => Some (TEnc true l t)
+  | _ => None
+  end.
+
+Definition dec k t : option term :=
+  match k, t with
+  | TKey KSym  l1, TEnc false l2 t
+  | TKey KADec l1, TEnc true  l2 t =>
+    if decide (l1 = l2) then Some t else None
+  | _, _ => None
+  end.
+
+Definition is_key t :=
+  match t with
+  | TKey kt _ => Some kt
+  | _ => None
+  end.
+
+End Spec.
